
%\renewcommand{\theequation}{\theenumi}
%\begin{enumerate}[label=\arabic*.,ref=\theenumi]
\begin{enumerate}[label=\thesection.\arabic*.,ref=\thesection.\theenumi]
%\begin{enumerate}
%\numberwithin{equation}{enumi}

\item Let 
\begin{align}
  \vec{A} &= \myvec{a_1\\a_2 \\ a_3} \equiv a_1\overrightarrow{i}+a_2\overrightarrow{j}+a_3\overrightarrow{j}, 
  \\
  \vec{B} &= \myvec{b_1\\b_2 \\ b_3}, 
\end{align}
and 
\begin{align}
  \vec{A}_{ij} &= \myvec{a_i\\a_j}, 
  \\
  \vec{B}_{ij} &= \myvec{b_i\\b_j}. 
\end{align}

\item The {\em cross product} or {\em vector product} of $\vec{A}, \vec{B}$ is defined as
\begin{align}
  \label{eq:cross3d}
	\vec{A} \times \vec{B} = \myvec{ \mydet{\vec{A}_{23} & \vec{B}_{23}} \\[10pt] \mydet{\vec{A}_{31} & \vec{B}_{31}} \\[10pt] \mydet{\vec{A}_{12}  & \vec{B}_{12}}}
\end{align}
\item Verify that
\begin{align}
  \vec{A} \times \vec{B} = -  \vec{B} \times \vec{A} 
\end{align}
\item The area of a triangle is given by 
\begin{align}
	\frac{1}{2} \norm{  \vec{A} \times \vec{B}}
\end{align}
\item (Cauchy-Schwarz Inequality)
    \begin{align}
        \label{eq:dot-mag-ineq}
	    \abs{\vec{a}^\top\vec{b}} &\le \norm{\vec{a}}\norm{\vec{b}}
    \end{align}
    \solution
	\begin{align}
        \norm{\vec{a}-\frac{\vec{a}^\top\vec{b}}{\norm{\vec{b}}^2}\vec{b}}^2 &\ge 0 \\
        \implies \norm{\vec{a}}^2 - 2\frac{\brak{\vec{a}^\top\vec{b}}^2}{\norm{\vec{b}}^2} + \frac{\brak{\vec{a}^\top\vec{b}}^2}{\norm{\vec{b}}^2} &\ge 0 \\
        \implies \norm{\vec{a}}^2 - \frac{\brak{\vec{a}^\top\vec{b}}^2}{\norm{\vec{b}}^2} &\ge 0 \\
        \implies \norm{\vec{a}}^2\norm{\vec{b}}^2 &\ge \brak{\vec{a}^\top\vec{b}}^2 \\
    \end{align}
    yielding
        \eqref{eq:dot-mag-ineq}.
\item (Triangle Inequality)
    \begin{align}
\norm{\vec{a}+\vec{b}} &\le \norm{\vec{a}}+\norm{\vec{b}}
        \label{eq:triangle-ineq}
    \end{align}
    \solution
    Using \eqref{eq:dot-mag-ineq},
    \begin{align}
        \vec{a}^\top\vec{b} &\le \norm{\vec{a}}\norm{\vec{b}} \\
\implies        \norm{\vec{a}}^2 + 2\vec{a}^\top\vec{b} + \norm{\vec{b}}^2 &\le \norm{\vec{a}}^2 + 2\norm{\vec{a}}\norm{\vec{b}} + \norm{\vec{b}}^2 \\
\implies               \norm{\vec{a}+\vec{b}}^2 &\le \brak{\norm{\vec{a}}+\norm{\vec{b}}}^2 
    \end{align}
    yielding
        \eqref{eq:triangle-ineq}.
\end{enumerate}
